use riscv-coq encoder to encode tiny assembly program and run it
on user-mode qemu-riscv32 (but without any memory yet)

src/Bedrock/Field/Synthesis/Examples/riscv/wrapper_template.s
@@ -1,0 +1,3 @@
+.section .text
+.globl _start
+_start: .incbin "FILENAME"
