src/Bedrock/Field/Synthesis/Examples/riscv/README.md
@@ -1,0 +1,34 @@
+## Running RISC-V programs compiled with the bedrock2 compiler in qemu user mode using system calls of the host OS
+
+### Prerequisites
+
+1) A RISC-V assembler & linker. On a Fedora Linux, I got it by installing all of the GNU RISC-V toolchain (but maybe there are more lightweight ways).
+
+```
+sudo dnf install autoconf automake python3 libmpc-devel mpfr-devel gmp-devel gawk  bison flex texinfo patchutils gcc gcc-c++ zlib-devel expat-devel
+mkdir /home/sam/installs/riscv-gnu-toolchain32/
+git clone --recursive git@github.com:riscv/riscv-gnu-toolchain.git
+cd ./riscv-gnu-toolchain
+./configure --prefix=/home/sam/installs/riscv-gnu-toolchain32 --with-arch=rv32ima --with-abi=ilp32
+make linux
+cd ~/installs/riscv-gnu-toolchain32/bin/
+export PATH=`pwd`:$PATH
+```
+
+2) qemu user mode emulator
+
+```
+sudo dnf install qemu-user
+```
+
+
+### Compiling & running
+
+Create a Coq file that outputs a hex dump of encoded instructions (eg `CompilerTest.v`), then run eg
+
+```
+make CompilerTest.exe
+qemu-riscv32 CompilerTest.exe
+```
+
+and use `echo $?` to check the exit code.
